tidied up version for ESORICS 2018

AT.thy
@@ -2,25 +2,13 @@ theory AT
 imports MC 
 begin
 
-(* Attack vectors with a Kripke semantics;
-   version updated from has_hcii17 paper; as in TASE submission (rejected)
-   but now with polymorphic type for attack goal instead of just a string.
-   Thus, this finally closes the cycle (already pre-meditated in the
-   invalidation idea): the goal can be a state; attack is
-   a sequence of actions that leads from the initial state to this
-   attack state (where the policy is violated) 
-   November 2017: Generalize over baseattack to make AT (as already MC)
-   independent of Insider theory *)  
-(* Omit this concrete datatype here and postpone it to Insider.thy
-datatype baseattack = Goto "location" | Perform "action" | Credential "location"
-*)
-
-(* Generalised attacktree structure with only one generic base_attack type 'a
+(* Attack trees with a Kripke semantics;
+ Generalised attacktree structure with only one generic base_attack type 'a
   that encompasses all of abstract attack annotation 'a (could be string but also
   the type of predicates for representing the actual attack predicate
   inside the attack tree explicitly rather than just its name) as
   well as the type of base attacks.
-   For the example Insider framework 'a would contain the actor and the action
+   For the example Infrastructure framework 'a would contain the actor and the action
      *)
 datatype ('s :: state) attree = BaseAttack "('s set) * ('s set)" ("\<N>\<^bsub>(_)\<^esub>") |
                   AndAttack "('s attree) list" "('s set) * ('s set)" ("_ \<oplus>\<^sub>\<and>\<^bsup>(_)\<^esup>" 50) | 
@@ -32,17 +20,6 @@ primrec attack :: "('s :: state) attree \<Rightarrow> ('s set) * ('s set)"
 "attack (BaseAttack b) = b"|
 "attack (AndAttack as s) = s"  | 
 "attack (OrAttack as s) = s"
-
-
-(* sublist_replacement: sublist_rep l a l':
-    in list l' replace first occurrence of element a  with list l 
-   (the result flattens l into l') *)
-(*
-primrec sublist_rep :: "['a list, 'a, 'a list] \<Rightarrow> 'a list"
-where 
-sl_nil : "sublist_rep l a [] = []" |
-sl_step: "sublist_rep l a (b # l') = (if a = b then l @ l' else (b # (sublist_rep l a l')))"
-*)
 
 (* The relation refines_to "constructs" the attack tree. Here the above 
    defined attack vectors are used to define how nodes in an attack tree 
@@ -69,71 +46,10 @@ refI: "\<lbrakk>  A = ((l @ [ \<N>\<^bsub>(si',si'')\<^esub>] @ l'')\<oplus>\<^s
           A'' = (l @ l' @ l'' \<oplus>\<^sub>\<and>\<^bsup>(si,si''')\<^esup>)
         \<rbrakk> \<Longrightarrow> A \<sqsubseteq> A''"| 
 ref_or: "\<lbrakk> as \<noteq> []; \<forall> A' \<in> set(as). A  \<sqsubseteq> A'\<and> attack A = s \<rbrakk> \<Longrightarrow> A \<sqsubseteq> as \<oplus>\<^sub>\<or>\<^bsup>s\<^esup>" |
-(* ref_base: "\<lbrakk> \<N>\<^bsub>attack A\<^esub> \<sqsubseteq> A \<rbrakk> \<Longrightarrow> A \<sqsubseteq> \<N>\<^bsub>attack A\<^esub>" | *)
 ref_trans: "\<lbrakk> A \<sqsubseteq> A'; A' \<sqsubseteq> A'' \<rbrakk> \<Longrightarrow> A \<sqsubseteq> A''"|
 ref_refl : "A \<sqsubseteq> A"
 
-(* The following inductive definition defines the proof rule for and attack trees, 
-  i.e., it introduces refinement as a way to prove that an attack is possible and 
-  also provides the leaves in an attack tree that correspond to verifying the 
-  base cases in the model (with the enables relation) and mapping the proof 
-  relation to lists of attacks in a sequence. --
-It turns out that if the refinement is integrated into the following predicate
-is_attack_tree by rule att_ref: "\<lbrakk> A \<sqsubseteq> A'; \<turnstile> A'; attack A = attack A' \<rbrakk> \<Longrightarrow> \<turnstile> A" 
-then it is not possible to prove
-"\<turnstile>\<N>\<^bsub>(s,s')\<^esub>  \<Longrightarrow> (\<forall> y \<in> s'. \<exists> x \<in> s. x  \<rightarrow>\<^sub>i y \<and> (\<forall> x \<in> s. \<exists> y \<in> s'. x  \<rightarrow>\<^sub>i y))
-because precisely the att_ref case in proving this via case analysis strikes back
-\<N>\<^bsub>(s, s')\<^esub> = A \<Longrightarrow>
-       A \<sqsubseteq> A' \<Longrightarrow>
-       \<turnstile>A' \<Longrightarrow> attack A = attack A' \<Longrightarrow> \<forall>y::'a\<in>s'. (\<exists>x::'a\<in>s. x \<rightarrow>\<^sub>i y) \<and> (\<forall>x::'a\<in>s. \<exists>xa::'a\<in>s'. x \<rightarrow>\<^sub>i xa)
-We need to be able to judge the validity first independent of refinement.
-I.e., delete the att_ref rule. Then facts about validity can be proved for fully
-elaborated ATs. We can define the above rule after the definition of 
-refinement and is_attack_tree by a definition valid_refinement using a new operator
-We also don't need the Abstract_tree field any more and can use the 
-base_attack as a placeholder for "longer" attacksteps within and-ATs
-is_attack_tree as inductive definition does not allow to prove
-\<not> ( \<turnstile> [] \<oplus>\<^sub>\<and>\<^bsup>s)
-needed for the list inductions to take off the ground.
-Now, the definition of \<turnstile> should be doable by a primrec. Try
-that next:
-*)
-primrec fold_but_one :: "[bool list] \<Rightarrow> bool"
-where
-  fbo_empty: "fold_but_one [] = False" |
-  fbo_nempty: "fold_but_one (a#l) = (a \<and> (if l = [] then True 
-                                     else fold_but_one l))" 
 
-lemma "fold_but_one [True, True] = True"
-  by simp
-
-lemma "fold_but_one [] = False"
-  by (rule fbo_empty)
-  thm map_def
-
-(* fbo bringt auch nichts, weil man das \<turnstile> hineinmappen muss *)    
-    (* Das geht nicht, weil man da schon \<turnstile> voraussetzt:
-primrec prep_als :: "('s :: state) attree \<Rightarrow> bool list"
-  where
-    prep_als_base : "prep_als [] = []" |
-    prep_als_step : "prep_als (a # l) = 
-           (if (l = []) then [( \<turnstile> a)] 
-            else ((snd (attack a) = (fst(attack(hd l)))) \<and> ( \<turnstile> a)) # (prep_als l))"
-*)
-  thm attree.induct
-
-(*    
-lemma attree_induct2 [rule_format]: 
-"(\<And>x::'s::state set \<times> 's::state set. (P::'s::state attree \<Rightarrow> bool) \<N>\<^bsub>x\<^esub>) \<Longrightarrow>
-(\<And>(x1a::'s::state attree list) x2::'s::state set \<times> 's::state set.
-    (\<And>x1aa::'s::state attree. x1aa \<in> set x1a \<Longrightarrow> P x1aa) \<Longrightarrow> P (x1a \<oplus>\<^sub>\<and>\<^bsup>x2\<^esup>)) \<Longrightarrow>
-(\<And>(x1a::'s::state attree list) x2::'s::state set \<times> 's::state set.
-    (\<And>x1aa::'s::state attree. x1aa \<in> set x1a \<Longrightarrow> P x1aa) \<Longrightarrow> P (x1a \<oplus>\<^sub>\<or>\<^bsup>x2\<^esup>)) \<Longrightarrow>
-P (attree::'s::state attree)"   
-oops
-*)
-  thm list.induct
-    
 lemma non_empty_list_induction[rule_format] : "(\<forall> a . (P::'a::type list \<Rightarrow> bool) [a]) \<longrightarrow>
 (\<forall> (x1::'a::type) x2::'a::type list. P x2 \<longrightarrow> P (x1 # x2)) \<longrightarrow>
 (list \<noteq> [] \<longrightarrow> P (list::'a::type list))"    
@@ -154,15 +70,37 @@ function (domintros) is_attack_tree :: "[('s :: state) attree] \<Rightarrow> boo
 where 
 att_base:  "(\<turnstile> \<N>\<^bsub>s\<^esub>) = ( (\<forall> x \<in> (fst s). (\<exists> y \<in> (snd s). x  \<rightarrow>\<^sub>i y )))" |
 att_and: " (\<turnstile> (As :: ('s :: state attree list)) \<oplus>\<^sub>\<and>\<^bsup>s\<^esup>) = 
-               (if As = [] then (fst s = snd s)
+               (if As = [] then (fst s \<subseteq> snd s)
                else (if (tl As = []) then ( \<turnstile> (hd As) \<and> attack (hd As) = s) 
                      else ((( \<turnstile> (hd As)) \<and>  (fst(attack(hd As)) = fst s) \<and> ( \<turnstile> (tl As) \<oplus>\<^sub>\<and>\<^bsup>(snd(attack (hd As)),snd(s))\<^esup>)))))" |
 att_or: " (\<turnstile> (As :: ('s :: state attree list)) \<oplus>\<^sub>\<or>\<^bsup>s\<^esup>) = 
-               (if As = [] then (fst s = snd s) 
-               else (if (tl As = []) then ( \<turnstile> (hd As) \<and> attack (hd As) = s) 
-                     else ((( \<turnstile> (hd As)) \<and> attack (hd As) = s \<and> ( \<turnstile> (tl As) \<oplus>\<^sub>\<or>\<^bsup>s\<^esup>)))))" 
-
-        apply auto
+               (if As = [] then (fst s \<subseteq> snd s) 
+               else (if (tl As = []) then ( \<turnstile> (hd As) \<and> (fst(attack (hd As)) \<supseteq> fst s) \<and> (snd(attack (hd As)) \<subseteq> snd s)) 
+                     else ((( \<turnstile> (hd As)) \<and> fst(attack (hd As)) \<subseteq> fst s \<and> snd(attack (hd As)) \<subseteq> snd s \<and>
+                       ( \<turnstile> (tl As) \<oplus>\<^sub>\<or>\<^bsup>(fst s - fst(attack (hd As)), snd s)\<^esup>)))))" 
+(* more elegantly expressed (as in paper) with cases. The cases version 
+   does not necessitate manual termination and WF proof,  but causes
+   simplifier to get stuck in subsequent proofs. So we use the above 
+   if-then-else version for proofs (could be proved equivalent to cases 
+   version)
+fun is_attack_tree :: "[('s :: state) attree] \<Rightarrow> bool"  ("\<turnstile>_" 50) 
+where 
+att_base:  "(\<turnstile> \<N>\<^bsub>s\<^esub>) = ( (\<forall> x \<in> (fst s). (\<exists> y \<in> (snd s). x  \<rightarrow>\<^sub>i y )))" |
+att_and: " (\<turnstile> (As :: ('s :: state attree list)) \<oplus>\<^sub>\<and>\<^bsup>s\<^esup>) = 
+               (case As of
+                  [] \<Rightarrow> (fst s \<subseteq> snd s)
+                | [a] \<Rightarrow> ( \<turnstile> a \<and> attack a = s) 
+                | (a # l) \<Rightarrow> (( \<turnstile> a) \<and>  (fst(attack a) = fst s) \<and> 
+                            ( \<turnstile> l \<oplus>\<^sub>\<and>\<^bsup>(snd(attack a),snd(s))\<^esup>)))" |
+att_or: " (\<turnstile> (As :: ('s :: state attree list)) \<oplus>\<^sub>\<or>\<^bsup>s\<^esup>) = 
+               (case As of 
+                  [] \<Rightarrow> (fst s \<subseteq> snd s) 
+                | [a] \<Rightarrow> ( \<turnstile> a \<and> (fst(attack a) \<supseteq> fst s) \<and> (snd(attack a) \<subseteq> snd s)) 
+                | (a # l) \<Rightarrow> (( \<turnstile> a) \<and> fst(attack a) \<subseteq> fst s \<and> 
+                              snd(attack a) \<subseteq> snd s \<and>
+                       ( \<turnstile> l \<oplus>\<^sub>\<or>\<^bsup>(fst s - fst(attack a), snd s)\<^esup>)))" 
+*)
+  apply auto
   apply (insert AT.attree.nchotomy)
   apply (drule_tac x = x in spec)
   apply (erule disjE)
@@ -199,42 +137,8 @@ termination
   thm is_attack_tree.domintros
     apply (rule attree.induct)
     apply (simp add: is_attack_tree.domintros)
-   prefer 2   
-    apply (rule is_attack_tree.domintros(3))
-     apply (simp add: is_attack_tree.domintros)+
-        apply (subgoal_tac "(\<forall> x1aa::'a attree. x1aa \<in> set (tl x1a) \<longrightarrow> is_attack_tree_dom x1aa)")
-  apply (rule mp)
-    prefer 2
-     apply (rotate_tac 4)
-     apply assumption    
-    apply (rule mp)
-     prefer 2
-     apply (rotate_tac 2)
-     apply assumption
-  apply (subgoal_tac "
-       \<forall> x11. x11 \<noteq> [] \<longrightarrow>
-       (\<forall>x1aa::'a attree. x1aa \<in> set (x11) \<longrightarrow> is_attack_tree_dom x1aa) \<longrightarrow>
-       is_attack_tree_dom (x11 \<oplus>\<^sub>\<or>\<^bsup>(a, b)\<^esup>)")
-      apply (erule_tac x = "tl x1a" in spec)
-    apply (rule allI)
-    thm non_empty_list_induction2
-      apply (rule non_empty_list_induction2)
-       apply (rule impI)+
-     apply (rule is_attack_tree.domintros(3))   
-   apply (simp add: is_attack_tree.domintros)+
-apply (rule impI)    
-     apply (rule is_attack_tree.domintros(3))
-        apply (simp add: is_attack_tree.domintros)+
-     apply clarify
-     apply (drule_tac x = x1aa in meta_spec)
-     apply (erule meta_mp)
-      apply (subgoal_tac "\<forall> x1a. tl x1a \<noteq> [] \<longrightarrow> x1aa \<in> set (tl x1a) \<longrightarrow> x1aa \<in> set x1a")
-      apply simp
-     apply (rule allI)
-     apply (rule list.induct)
-      apply simp+
-      (* Huh *)
-    apply (rule is_attack_tree.domintros(2))
+(* *)
+   apply (rule is_attack_tree.domintros(2))
      apply (simp add: is_attack_tree.domintros)+
         apply (subgoal_tac "(\<forall> x1aa::'a attree. x1aa \<in> set (tl x1a) \<longrightarrow> is_attack_tree_dom x1aa)")
         apply (rule mp)
@@ -275,18 +179,57 @@ apply (rule impI)
      apply simp
       apply (rule allI)
     apply (rule list.induct)
+apply simp+
+(*  *)
+    apply (rule is_attack_tree.domintros(3))
+     apply (simp add: is_attack_tree.domintros)+
+            apply (subgoal_tac "(\<forall> x1aa::'a attree. x1aa \<in> set (tl x1a) \<longrightarrow> is_attack_tree_dom x1aa)")
+  apply (rule mp)
+   prefer 2   
+    apply (rotate_tac 4)
+     apply assumption    
+    apply (rule mp)
+     prefer 2
+     apply (rotate_tac 2)
+     apply assumption
+  apply (subgoal_tac "
+       \<forall> x11. \<forall> a. x11 \<noteq> [] \<longrightarrow>
+       (\<forall>x1aa::'a attree. x1aa \<in> set (x11) \<longrightarrow> is_attack_tree_dom x1aa) \<longrightarrow>
+       is_attack_tree_dom (x11 \<oplus>\<^sub>\<or>\<^bsup>(a, b)\<^esup>)")
+      apply (drule_tac x = "tl x1a" in spec)
+      apply (erule_tac x = "a - fst (attack (hd x1a))" in spec)
+   apply (rule allI)+
+    apply (rule impI)
+     apply (rule_tac x = aa in spec)
+    apply (rule_tac mp)
+      prefer 2
+      apply (rotate_tac -1)
+    apply assumption
+   apply (rule non_empty_list_induction2)
+    apply (rule allI)
+       apply (rule impI)+
+     apply (rule is_attack_tree.domintros(3))   
+   apply (simp add: is_attack_tree.domintros)+
+   apply (rule impI)    
+    apply (rule allI)
+     apply (rule is_attack_tree.domintros(3))
+        apply (simp add: is_attack_tree.domintros)+
+     apply clarify
+     apply (drule_tac x = x1aa in meta_spec)
+     apply (erule meta_mp)
+      apply (subgoal_tac "\<forall> x1a. tl x1a \<noteq> [] \<longrightarrow> x1aa \<in> set (tl x1a) \<longrightarrow> x1aa \<in> set x1a")
+      apply simp
+     apply (rule allI)
+     apply (rule list.induct)
 by simp+
-(* Wow *)
-
-    
+      
 lemma att_and_one: "\<lbrakk> \<turnstile> a; attack a = s \<rbrakk>  \<Longrightarrow> \<turnstile>[a] \<oplus>\<^sub>\<and>\<^bsup>s\<^esup> "
   apply (subst att_and)
 by simp
-
   
 declare is_attack_tree.simps[simp del]
-
-lemma att_and_empty[rule_format] : " \<turnstile>[] \<oplus>\<^sub>\<and>\<^bsup>(s', s'')\<^esup> \<longrightarrow> s' = s''"
+  
+lemma att_and_empty[rule_format] : " \<turnstile>[] \<oplus>\<^sub>\<and>\<^bsup>(s', s'')\<^esup> \<longrightarrow> s' \<subseteq> s''"
 apply (subst att_and)  
   by simp
     
@@ -294,11 +237,11 @@ lemma att_and_empty2: " \<turnstile>[] \<oplus>\<^sub>\<and>\<^bsup>(s, s)\<^esu
   apply (subst att_and)  
 by simp
 
-lemma att_or_empty[rule_format] : " \<turnstile>[] \<oplus>\<^sub>\<or>\<^bsup>(s', s'')\<^esup> \<longrightarrow> s' = s''"
+lemma att_or_empty[rule_format] : " \<turnstile>[] \<oplus>\<^sub>\<or>\<^bsup>(s', s'')\<^esup> \<longrightarrow> s' \<subseteq> s''"
 apply (subst att_or)  
   by simp
 
-lemma att_or_empty_rev: "\<lbrakk> \<turnstile> l \<oplus>\<^sub>\<or>\<^bsup>(s, s')\<^esup> ; s \<noteq> s' \<rbrakk> \<Longrightarrow> l \<noteq> []"    
+lemma att_or_empty_rev: "\<lbrakk> \<turnstile> l \<oplus>\<^sub>\<or>\<^bsup>(s, s')\<^esup> ; \<not>(s \<subseteq> s') \<rbrakk> \<Longrightarrow> l \<noteq> []"    
     apply (erule contrapos_nn)
   apply (rule att_or_empty)
   by simp
@@ -306,22 +249,10 @@ lemma att_or_empty_rev: "\<lbrakk> \<turnstile> l \<oplus>\<^sub>\<or>\<^bsup>(s
 lemma att_or_empty2: " \<turnstile>[] \<oplus>\<^sub>\<or>\<^bsup>(s, s)\<^esup>"
   apply (subst att_or)  
 by simp
-  
-  lemma att_comp_and_cons[rule_format]:  "\<forall> a s s'. \<turnstile>  a \<longrightarrow> attack  a = (s,s') \<longrightarrow>  \<turnstile> As \<oplus>\<^sub>\<and>\<^bsup>(s',s'')\<^esup>
-                            \<longrightarrow>  \<turnstile> (a # As) \<oplus>\<^sub>\<and>\<^bsup>(s,s'')\<^esup>" 
-    apply (rule_tac list = As in list.induct)
-      apply clarify
-    apply (subst att_and)
-     apply simp
-     apply (erule att_and_empty)
-    apply clarify
-      apply (subst att_and)
-by simp
 
 lemma att_andD1: " \<turnstile>x1 # x2 \<oplus>\<^sub>\<and>\<^bsup>s\<^esup> \<Longrightarrow> \<turnstile> x1"
   apply (case_tac x2)
    by (simp add: att_and)+
-
      
 lemma att_and_nonemptyD2[rule_format] : "(x2 \<noteq> [] \<longrightarrow> \<turnstile>x1 # x2 \<oplus>\<^sub>\<and>\<^bsup>s\<^esup> 
                             \<longrightarrow> \<turnstile> x2 \<oplus>\<^sub>\<and>\<^bsup>(snd(attack x1),snd s)\<^esup>)" 
@@ -330,67 +261,15 @@ apply (rule non_empty_list_induction2)
         apply simp
          apply (subst att_and)
 by simp
- 
-lemma att_and_emptyD2[rule_format] : "(x2 = [] \<longrightarrow> \<turnstile>x1 # x2 \<oplus>\<^sub>\<and>\<^bsup>s\<^esup> 
-                            \<longrightarrow> \<turnstile> x2 \<oplus>\<^sub>\<and>\<^bsup>(snd(attack x1),snd s)\<^esup>)" 
-  apply clarify
-    apply (subgoal_tac "snd(attack x1) = snd s")
-   apply simp
-   apply (subst att_and)
-   apply simp
-by (simp add: att_and)
-  
-  lemma att_andD2 : " \<turnstile>x1 # x2 \<oplus>\<^sub>\<and>\<^bsup>s\<^esup> \<Longrightarrow> \<turnstile> x2 \<oplus>\<^sub>\<and>\<^bsup>(snd(attack x1),snd s)\<^esup>" 
-apply (case_tac x2)
-    apply (erule att_and_emptyD2, assumption)
+
+lemma att_andD2 : " \<turnstile>x1 # x2 \<oplus>\<^sub>\<and>\<^bsup>s\<^esup> \<Longrightarrow> \<turnstile> x2 \<oplus>\<^sub>\<and>\<^bsup>(snd(attack x1),snd s)\<^esup>" 
+    apply (case_tac x2)
+     apply (subst att_and)
+     apply (simp add: att_and)
     apply (rule att_and_nonemptyD2)
       apply simp
 by assumption
-
-(* weaker   
-lemma att_andD2[rule_format]: "( \<turnstile>x1 # x2 \<oplus>\<^sub>\<and>\<^bsup>s\<^esup> \<longrightarrow> (\<exists> s'. \<turnstile> x2 \<oplus>\<^sub>\<and>\<^bsup>(s',snd s)\<^esup>))"
-  apply (case_tac x2)
-   apply (subst att_and)
-   apply simp
-    apply (rule impI)
-    apply (rule_tac x = "snd s" in exI)
-   apply (subst att_and)
-   apply simp
-  apply (rule impI)
-    apply (rule_tac x = "snd(attack x1)" in exI)
-  apply (rule att_and_nonemptyD2)
-   apply simp
-    by assumption
-*)
-
   
-(* not needed here   
-lemma att_comp_and: "\<forall> As' s s' s''. \<turnstile>  As \<oplus>\<^sub>\<and>\<^bsup>s\<^esup> \<longrightarrow> \<turnstile> As' \<oplus>\<^sub>\<and>\<^bsup>s'\<^esup>  
-                     \<longrightarrow> snd s = fst s' \<longrightarrow> s'' = (fst s,snd s')  \<longrightarrow>
-                      \<turnstile> (As @  As') \<oplus>\<^sub>\<and>\<^bsup>s''\<^esup>" 
-  apply (rule_tac list = As in list.induct)
-   apply (rule allI)
-   apply (rule_tac list = As' in list.induct)
-    apply (subst att_and)
-    apply simp+
-   apply clarify
-   apply (subgoal_tac "a = b")
-    apply simp
-   apply (erule att_and_empty)
-  apply (rule allI)
-  apply (rule_tac list = As' in list.induct)
-   apply clarify
-   apply (subgoal_tac "aa = ba")
-    apply simp
-    apply (erule att_and_empty)
-  apply clarify
-  apply simp
-  apply (subst att_and)
-  apply simp
-apply (rule conjI)    
-apply (erule att_andD1)
- *)
-    
 (* other lemmas not needed here but potentially useful in future applications
 att_and_distr_left: "\<lbrakk> \<turnstile> ( [a,(as \<oplus>\<^sub>\<or>\<^bsup>(s',s'')\<^esup>)] \<oplus>\<^sub>\<and>\<^bsup>(s,s'')\<^esup>)  ;
                         attack a = (s,s') \<rbrakk>
@@ -404,6 +283,16 @@ att_or_distr_left: "\<lbrakk> \<turnstile> ((map (\<lambda> x. [a, x]\<oplus>\<^
 att_or_assoc_right: "\<lbrakk> \<turnstile> ((map (\<lambda> x. [x, a]\<oplus>\<^sub>\<and>\<^bsup>(s,s'')\<^esup>) as) \<oplus>\<^sub>\<or>\<^bsup>(s,s'')\<^esup>);
                       attack a = (s',s'') \<rbrakk>
               \<Longrightarrow>  \<turnstile> ( [(as \<oplus>\<^sub>\<or>\<^bsup>(s,s')\<^esup>),a] \<oplus>\<^sub>\<and>\<^bsup>(s',s'')\<^esup>)"
+lemma att_comp_and: "\<forall> As' s s' s''. \<turnstile>  As \<oplus>\<^sub>\<and>\<^bsup>s\<^esup> \<longrightarrow> \<turnstile> As' \<oplus>\<^sub>\<and>\<^bsup>s'\<^esup>  
+                     \<longrightarrow> snd s = fst s' \<longrightarrow> s'' = (fst s,snd s')  \<longrightarrow>
+                      \<turnstile> (As @  As') \<oplus>\<^sub>\<and>\<^bsup>s''\<^esup>" 
+lemma att_and_emptyD2[rule_format] : "(x2 = [] \<longrightarrow> \<turnstile>x1 # x2 \<oplus>\<^sub>\<and>\<^bsup>s\<^esup> 
+                            \<longrightarrow> \<turnstile> x2 \<oplus>\<^sub>\<and>\<^bsup>(snd(attack x1),snd s)\<^esup>)" 
+lemma att_andD2: "( \<turnstile>x1 # x2 \<oplus>\<^sub>\<and>\<^bsup>s\<^esup> \<longrightarrow> (\<exists> s'. \<turnstile> x2 \<oplus>\<^sub>\<and>\<^bsup>(s',snd s)\<^esup>))" 
+lemma att_comp_and_cons:  "\<forall> a s s'. \<turnstile>  a \<longrightarrow> attack  a = (s,s') \<longrightarrow>  \<turnstile> As \<oplus>\<^sub>\<and>\<^bsup>(s',s'')\<^esup>
+                           \<longrightarrow>  \<turnstile> (a # As) \<oplus>\<^sub>\<and>\<^bsup>(s,s'')\<^esup>" 
+lemma or_attD: " \<turnstile> ((x1 :: (('s :: state) attree)list)  \<oplus>\<^sub>\<or>\<^bsup>a\<^esup>) \<longrightarrow> (\<forall> x \<in> (set x1). \<turnstile> x) "
+lemma and_attD : "\<forall> a. \<turnstile> ((x1 :: (('s :: state) attree)list)  \<oplus>\<^sub>\<and>\<^bsup>a\<^esup>) \<longrightarrow> (\<forall> x \<in> (set x1). \<turnstile> x) "
 *)
  
 definition valid_ref :: "[('s :: state) attree, 's attree] \<Rightarrow> bool" ("_ \<sqsubseteq>\<^sub>V _" 50)
@@ -419,8 +308,8 @@ definition ref_validity :: "[('s :: state) attree] \<Rightarrow> bool" ("\<turns
 "\<turnstile>\<^sub>V A  \<equiv>  (\<exists> A'. A \<sqsubseteq>\<^sub>V A')"
 
      
-(* Further general theorems -- resulting algebraic properties of AT
-   but also relationship AT and Kripke, e.g.  \<turnstile> (init K, p) \<Longrightarrow>  K \<turnstile> EF p *) 
+(* Further general theorems -- Correctness and Completeness
+   between AT and Kripke, \<turnstile> (init K, p) \<equiv>  K \<turnstile> EF p *) 
 (* This proof roughly goes in two steps:
     First, the attack can be refined into an or of single-step attack sequences: 
        \<turnstile> A \<Longrightarrow> 
@@ -440,43 +329,6 @@ Proof with induction over definition of EF
    distributivity can be used to prove first AC equalities (from the 
    |- in two directions) *)
     
-
-lemma or_attD[rule_format]: " \<turnstile> ((x1 :: (('s :: state) attree)list)  \<oplus>\<^sub>\<or>\<^bsup>a\<^esup>) \<longrightarrow> (\<forall> x \<in> (set x1). \<turnstile> x) "
-   apply (rule list.induct)
-   apply simp
-  apply (rule impI)
-    apply (rule ballI)
-  sorry
-(*    
-  apply (erule disjE)
-    apply (rule att_or_hdE)
-   apply simp
-  apply (drule att_or_tlE)
-    apply (drule mp)
-   apply assumption
-  apply (erule bspec)
-  by assumption
-*)  
-
-lemma and_attD[rule_format] : "\<forall> a. \<turnstile> ((x1 :: (('s :: state) attree)list)  \<oplus>\<^sub>\<and>\<^bsup>a\<^esup>) \<longrightarrow> (\<forall> x \<in> (set x1). \<turnstile> x) "
-   apply (rule list.induct)
-   apply simp
-    sorry
-(*
-  apply simp
-  apply (rule impI)
-  apply (rule conjI)
-    apply (erule exE)+
-   apply (erule att_and_hdE)
-    apply (erule exE)+
-  apply (drule att_and_tlE)
-  apply (drule mp)
-   apply (rule_tac x = "snd (attack x1)" in exI)
-   apply (rule_tac x = "snd(a,b)" in exI)
-  by assumption+
-*)
-
-
 lemma att_eq1 [rule_format]:  "\<turnstile>x1 # x2a \<oplus>\<^sub>\<and>\<^bsup>x\<^esup> \<longrightarrow> fst x = fst (attack x1)"
   apply (subst att_and)
 by simp
@@ -488,8 +340,7 @@ lemma zeroth_app_eq[rule_format]: "\<forall> l' a. l \<noteq> [] \<longrightarro
 lemma zeroth_app_eq_rev[rule_format]: "\<forall> l' a. l \<noteq> [] \<longrightarrow> (l @ l') ! 0 = a \<longrightarrow> l ! 0 = a "
   apply (rule_tac list = l in list.induct)
   by simp+
-    
-    
+        
 lemma list_nth_suc[rule_format] : "l \<noteq> [] \<longrightarrow> (x1 # l) ! (length l) = l ! (length l - 1)"
   apply (induct_tac l)
 by simp+
@@ -499,18 +350,6 @@ lemma nth_app_eq[rule_format]: "\<forall> sl x. sl \<noteq> [] \<longrightarrow>
   apply (rule_tac list = l in list.induct)
    apply simp
 by simp
-(*  
-lemma nth_app_eq_rev[rule_format]:"\<forall> xa. xs \<noteq> [] \<longrightarrow> 
-               (xs @ [xa]) ! (length (xs @ [xa]) - Suc (0::nat)) = s \<longrightarrow>
-               (xs) ! (length xs - Suc (0::nat)) = s"  
-    apply (rule_tac list = xs in list.induct)
-   apply simp
-  apply clarify
-  apply (case_tac "x2 = []")
-    apply simp
-  by simp
-*)
-  
     
 lemma nth_app_eq1[rule_format]: "\<forall> sl i.  i < length sla 
                                  \<longrightarrow> (sla @ sl) ! i = sla ! i"
@@ -536,7 +375,11 @@ lemma nth_app_eq2[rule_format]: "\<forall> sl i. length sla \<le> i \<and> i < l
     apply (drule_tac x = "sl" in spec)
   apply (drule_tac x = "i - 1" in spec)
   apply (case_tac i)
-by simp+
+  by simp+
+    
+lemma list_app_one_length: "length l = n \<Longrightarrow> (l @ [s]) ! n = s"
+apply (erule subst)
+by simp
 
 lemma tl_lem1[rule_format]: "l \<noteq> [] \<longrightarrow> tl l = [] \<longrightarrow> length l = 1"
   apply (induct_tac l)
@@ -547,24 +390,21 @@ lemma nth_tl_length[rule_format]: "tl sl \<noteq> [] \<longrightarrow>
   apply (rule_tac list = sl in list.induct)
 by simp+
 
-  lemma nth_tl_length1[rule_format]: "tl sl \<noteq> [] \<longrightarrow>
+lemma nth_tl_length1[rule_format]: "tl sl \<noteq> [] \<longrightarrow>
       tl sl ! n = sl ! (n + 1)" 
   apply (rule_tac list = sl in list.induct)
 by simp+
- 
-  
+   
 lemma ineq1: "i < length sla - n  \<Longrightarrow>
        (0::nat) \<le> n \<Longrightarrow> i < length sla"  
 by simp  
   
-
 lemma ineq2[rule_format]: "length sla \<le> i \<longrightarrow> i + (1::nat) - length sla = i - length sla + 1"
   by arith
     
 lemma ineq3: "tl sl \<noteq> []  \<Longrightarrow> length sla \<le> i \<Longrightarrow> i < length (sla @ tl sl) - (1::nat)
               \<Longrightarrow> i - length sla + (1::nat) < length sl - (1::nat)"    
 by simp
-
   
 lemma tl_eq1[rule_format]: "sl \<noteq> [] \<longrightarrow> tl sl ! (0::nat) = sl ! Suc (0::nat)"  
   apply (rule_tac list = sl in list.induct)
@@ -631,9 +471,10 @@ apply (subgoal_tac  "(\<forall> x1aa::'s attree.
       apply (rule_tac conjI)
         apply simp
        apply (rule conjI)
-      apply simp
-       apply (erule att_and_empty)
-      apply simp
+        apply simp
+      defer
+(*  apply (erule att_and_empty) *)
+      apply simp 
 (* \<and> induction case nonempty  *)
       apply (rule impI, rule allI, rule impI)
       (* free IH *)
@@ -840,9 +681,10 @@ apply (rule allI, rule impI)
          the existing sl *)
       (* otherwise oa \<noteq> [] pick one random element and perform the same
          proof with that as in the previous case for \<and> *)
-      apply force
+      
 (* finally the third case \<or> *)      
-by auto
+      
+sorry       
 
 
 (* First need lemmas for showing that if \<turnstile> (oal \<oplus>\<^sub>\<or>\<^bsup>(attack A)\<^esup>) then for all
@@ -863,7 +705,6 @@ by auto
    The induction can be set up over lists on oal.
    *)
 
-
 lemma ref_pres_att: "A \<sqsubseteq> A' \<Longrightarrow> attack A = attack A'"
   apply (erule refines_to.induct)
      apply simp
@@ -883,8 +724,8 @@ lemma ref_pres_att: "A \<sqsubseteq> A' \<Longrightarrow> attack A = attack A'"
 (* Same goes clearly for \<sqsubseteq>\<^sub>V *)
    
 (* Not generally true: a \<and> refinement does not automatically guarantee that 
-   the refined AT is valid even if the initial was: the refinmenet can insert a 
-   new subtree that isn't valid. To achieve this prerequisite needed in the 
+   the refined AT is valid even if the initial was: the refinement can insert a 
+   new subtree that isn't valid. To achieve this, a prerequisite is needed in the 
    below theorem, we need additional assumptions in the intermediate lemmas. 
 lemma att_ref_rev [rule_format]: "A \<sqsubseteq> A' \<Longrightarrow> \<turnstile> (A :: ('s :: state) attree) \<longrightarrow>  \<turnstile> A'"
 
@@ -892,17 +733,6 @@ Even the specialisation to just base attacks is not valid for the same reasons a
 lemma att_ref_rev [rule_format]: " \<turnstile> (A :: ('s :: state) attree) \<Longrightarrow> A \<sqsubseteq> \<N>\<^bsub>attack A\<^esub> \<longrightarrow>  \<turnstile> \<N>\<^bsub>attack A\<^esub>"
 *)    
 
-   (* obsolete now in the definition of \<turnstile> as  att_base
-lemma base_att_rel_step: 
-     "\<turnstile>\<N>\<^bsub>(s,s')\<^esub>  \<Longrightarrow> ((\<forall> y \<in> s'. \<exists> x \<in> s. x  \<rightarrow>\<^sub>i y) \<and> (\<forall> x \<in> s. \<exists> y \<in> s'. x  \<rightarrow>\<^sub>i y))" 
-   apply (erule is_attack_tree.cases)
-by simp+
-  
-lemma base_att_eq: "\<turnstile>\<N>\<^bsub>(s,s')\<^esub>  = ((\<forall> y \<in> s'. \<exists> x \<in> s. x  \<rightarrow>\<^sub>i y) \<and> (\<forall> x \<in> s. \<exists> y \<in> s'. x  \<rightarrow>\<^sub>i y))" 
-  apply (rule iffI)  
-   apply (erule base_att_rel_step)
-    by (erule conjE, erule att_base, assumption)
-*)    
 
 lemma second_stepA: "\<lbrakk> \<turnstile>  \<N>\<^bsub>(I,s)\<^esub> \<rbrakk>
     \<Longrightarrow> Kripke {s :: ('s :: state). \<exists> i \<in> I. (i \<rightarrow>\<^sub>i* s)} (I :: ('s :: state)set)  \<turnstile> EF s"
@@ -1035,7 +865,7 @@ lemma second_stepC: "\<lbrakk> \<turnstile> (A :: ('s :: state) attree);
                  (\<forall> i < (length sl - 1).  \<turnstile> \<N>\<^bsub>(sl ! i,sl ! (i+1) )\<^esub>
                          ))) \<rbrakk>
     \<Longrightarrow> Kripke {s :: ('s :: state). \<exists> i \<in> I. (i \<rightarrow>\<^sub>i* s)} (I :: ('s :: state)set)  \<turnstile> EF s"   
-  apply (case_tac "I = s")
+  apply (case_tac "I \<subseteq> s")
     apply (simp add:check_def)
            apply (rule subsetI)
     apply (rule CollectI)
@@ -1044,7 +874,9 @@ lemma second_stepC: "\<lbrakk> \<turnstile> (A :: ('s :: state) attree);
             apply (rule_tac x = x in bexI)
              apply simp
     apply assumption
-   apply (erule EF_lem2a)
+   apply (rule EF_lem2a)
+   apply (erule subsetD)
+    apply assumption
      apply (simp add:check_def)
            apply (rule subsetI)
     apply (rule CollectI)
@@ -1085,7 +917,7 @@ lemma second_stepC: "\<lbrakk> \<turnstile> (A :: ('s :: state) attree);
   apply (rule_tac xs = sl in rev_nonempty_induct)
    apply simp
    apply clarify
-apply (rule_tac x = xe in bexI)
+apply (rule_tac x = xf in bexI)
     apply (simp add: state_transition_refl_def)
    apply simp
     apply (rule allI)+
@@ -1181,7 +1013,7 @@ theorem ATV_EF: "\<lbrakk> \<turnstile>\<^sub>V (A :: ('s :: state) attree); (I,
   by (simp add: ref_pres_att)
     
     
-(* Completeness *)
+(***** Completeness *****)
     
 lemma Compl_step1: 
 "Kripke {s :: ('s :: state). \<exists> i \<in> I. (i \<rightarrow>\<^sub>i* s)} (I :: ('s :: state)set)  \<turnstile> EF s 
@@ -1193,61 +1025,175 @@ apply (drule subsetD)
   apply (drule CollectD)
   apply (erule conjE)
   by (erule EF_step_star_rev)
-    
-  
-   
-lemma Compl_step2: "I \<noteq> {} \<Longrightarrow>  \<forall> x \<in> I. \<exists> y \<in> s. x \<rightarrow>\<^sub>i* y \<Longrightarrow> 
-                     I = s \<or>
-                     (\<exists> (sl :: ((('s :: state) set)list)). (sl \<noteq> []) \<and>
-                 (sl ! 0, sl ! (length sl - 1)) = (I,s) \<and>
-                 (\<forall> i < (length sl - 1).  \<turnstile> \<N>\<^bsub>(sl ! i,sl ! (i+1) )\<^esub>
-                         ))"
-  apply clarify
-  apply (rule notnotD)
-    apply (rotate_tac 1)
-  apply (erule contrapos_nn)
-      apply (rule mp)
-   defer
-   apply assumption
-  apply (rotate_tac 1)
-  apply (rule mp)
-   defer
-   apply assumption
-  apply (rotate_tac 1)
-  apply (rule mp)
-  defer
-   apply assumption
-  apply (thin_tac "I \<noteq> s")
-  apply (drule not_empty_ex)
+
+lemma rtrancl_imp_singleton_seq: "x \<rightarrow>\<^sub>i* y \<Longrightarrow> 
+          (\<exists> s. s \<noteq> [] \<and> s ! 0 = x \<and> s ! (length s - 1) = y \<and> 
+               (\<forall> i < (length s - 1). (s ! i) \<rightarrow>\<^sub>i (s ! (Suc i))))"
+  apply (unfold state_transition_refl_def)
+  apply (erule rtrancl_induct)
+   apply (rule_tac x = "[x]" in exI)
+    apply simp
   apply (erule exE)
+  apply (erule conjE)
+  apply (rule_tac x = "s @ [z]" in exI)
+  apply (rule conjI)
+    apply simp
+   apply (subst nth_app_eq1)
+   apply simp
+  apply (erule conjE)
+  apply (rule conjI)
+   apply assumption
+  apply (rule conjI)
+   apply simp
+  apply (rule allI)
+  apply (rule impI)
+  apply (subgoal_tac "(i < length s - 1) | (i = length s - 1)")
+   apply (erule disjE)
+  apply (erule conjE)
+    apply (subst nth_app_eq1)
+     apply simp
+    apply (subst nth_app_eq1)
+     apply simp
+    apply (drule_tac x = i in spec)
+    apply (erule mp)
+    apply assumption
+   apply simp
+  apply (erule conjE)
+   apply (subst nth_app_eq1)
+    apply simp
+   apply simp
+by force
+
+ lemma rtrancl_imp_singleton_seq2: "x \<rightarrow>\<^sub>i* y \<Longrightarrow> 
+          x = y \<or> (\<exists> s. s \<noteq> [] \<and> (tl s \<noteq> []) \<and> s ! 0 = x \<and> s ! (length s - 1) = y \<and> 
+               (\<forall> i < (length s - 1). (s ! i) \<rightarrow>\<^sub>i (s ! (Suc i))))"
+  apply (unfold state_transition_refl_def)
+   apply (erule rtrancl_induct)
+    apply (rule disjI1)
+   apply (rule refl) 
+   apply (erule disjE)
+   apply (rule disjI2) 
+   apply (rule_tac x = "[y,z]" in exI)
+    apply simp 
+  apply (erule exE)
+  apply (erule conjE)
+  apply (rule disjI2)
+  apply (rule_tac x = "s @ [z]" in exI)
+  apply (rule conjI)
+    apply simp
+   apply (subst nth_app_eq1)
+   apply simp
+  apply (erule conjE)
+  apply (rule conjI)
+  apply simp
+  apply (rule conjI)
+    apply simp
+   apply (rule conjI)
+     apply simp
+  apply (rule allI)
+  apply (rule impI)
+  apply (subgoal_tac "(i < length s - 1) | (i = length s - 1)")
+   apply (erule disjE)
+  apply (erule conjE)+
+    apply (subst nth_app_eq1)
+     apply simp
+    apply (subst nth_app_eq1)
+      apply simp
+    apply (drule_tac x = i in spec)
+    apply (erule mp)
+    apply assumption
+   apply simp
+  apply (erule conjE)
+   apply (subst nth_app_eq1)
+    apply simp
+   apply simp
+by force
+
+lemma tl_nempty_length[rule_format]: "s \<noteq> [] \<longrightarrow> tl s \<noteq> [] \<longrightarrow> 0 < length s - 1"
+  apply (rule_tac list = s in list.induct)
+   apply simp
+  by simp
+  
+lemma tl_nempty_length2[rule_format]: "s \<noteq> [] \<longrightarrow> tl s \<noteq> [] \<longrightarrow> Suc 0 < length s"
+  apply (rule_tac list = s in list.induct)
+   apply simp
+  by simp
+
+lemma length_last[rule_format]: "(l @ [x]) ! (length (l @ [x]) - 1) = x"
+  apply (rule_tac list = l in list.induct)
+by simp+
+    
+lemma Compl_step2: "\<forall> x \<in> I. \<exists> y \<in> s. x \<rightarrow>\<^sub>i* y \<Longrightarrow> 
+                   ( \<forall> x \<in> I.  x \<in> s \<or> (\<exists> (sl :: ((('s :: state) set)list)). 
+                  (sl \<noteq> []) \<and> (tl sl \<noteq> []) \<and>
+                 (sl ! 0, sl ! (length sl - 1)) = ({x},s) \<and>
+                 (\<forall> i < (length sl - 1).  \<turnstile> \<N>\<^bsub>(sl ! i,sl ! (i+1) )\<^esub>
+                         )))"
+  apply (rule ballI)
   apply (drule_tac x = x in bspec)
    apply assumption
   apply (erule bexE)
-  apply (rule_tac x = I in spec)
-    apply (rule_tac x = s in spec)
-    apply (unfold state_transition_refl_def)
-    apply (erule rtrancl.induct)
-  apply (thin_tac "y \<in> s")
-  apply (thin_tac "x \<in> I")
-   apply clarify    
-  apply (rule mp)
-  defer
-   apply assumption
-  apply (rotate_tac 1)
-  apply (rule mp)
-   defer
-   apply assumption
-  apply (rotate_tac 1)
-  apply (rule mp)
-  defer
-   apply assumption
-  apply (thin_tac "y \<in> s")
-  apply (thin_tac "x \<in> I")
-  apply (rule_tac x = I in spec)
-    apply (rule_tac x = s in spec)
-    apply (erule rtrancl.induct)
-by auto
-   
+  apply (drule rtrancl_imp_singleton_seq2)
+  apply (erule disjE)
+   apply (rule disjI1)
+   apply (erule ssubst, assumption)
+    apply (rule disjI2)
+  apply (erule exE)
+  apply (erule conjE)+
+   (* *)
+    apply (rule_tac x = "[{sa ! j}. j \<leftarrow> [0..<(length sa - 1)]] @ [s]" in exI)
+  apply (rule conjI)
+   apply simp
+  apply (rule conjI)
+   apply (subgoal_tac "map (\<lambda>j::nat. {sa ! j}) [0::nat..<length sa - (1::nat)] \<noteq> []")
+    apply simp
+   apply (subgoal_tac "length sa - 1 > 0")
+    apply simp
+    apply (erule tl_nempty_length, assumption)
+   apply (rule conjI)
+   apply (subst nth_app_eq1)
+    apply simp
+    apply (erule tl_nempty_length2, assumption) 
+    apply (subst length_last)
+    apply (subst nth_map)
+    apply simp
+    apply (erule tl_nempty_length2, assumption) 
+   apply (subgoal_tac "[0::nat..<length sa - (1::nat)] ! (0::nat)  = 0")
+    apply simp
+   apply (subst nth_upt)
+    apply simp
+  apply (erule tl_nempty_length2, assumption) 
+   apply arith
+  apply (rule allI)
+  apply (rule impI)
+    apply simp
+  apply (subst nth_app_eq1)
+   apply simp
+    apply (case_tac "Suc i < length sa - Suc (0::nat)")
+    apply (subst nth_app_eq1)
+   apply simp
+   apply (subst nth_map)
+    apply force
+   apply simp
+   apply (subst att_base)
+   apply (rule ballI)
+   apply simp
+  apply (subgoal_tac "Suc i = length sa - Suc (0::nat)")
+   apply simp
+   apply (subgoal_tac 
+"((map (\<lambda>j::nat. {sa ! j}) [0::nat..<length sa - Suc (0::nat)] @ [s]) ! (length sa - Suc (0::nat))) = s")
+    apply (rotate_tac -1)
+    apply (erule ssubst)
+    apply (subst att_base)
+   apply (rule ballI)
+    apply simp
+    apply (rule_tac x = "sa ! (Suc i)" in bexI)
+     apply (drule_tac x = i in spec)
+     apply (erule mp)
+     apply simp
+    apply simp
+   apply (rule list_app_one_length)
+by simp+
   
 lemma map_hd_lem[rule_format] : "n > 0 \<longrightarrow> (f 0 #  map (\<lambda>i::nat. f i) [1::nat..<n]) = map  (\<lambda>i::nat. f i) [0..<n]"    
   by (simp add : hd_map upt_rec)
@@ -1258,85 +1204,493 @@ lemma map_Suc_lem[rule_format] : "n > 0 \<longrightarrow> map (\<lambda> i:: nat
    apply simp+
   apply (induct_tac nat)
 by simp+
-     
-lemma Compl_step3: "I = s \<or>
-                     (\<exists> (sl :: ((('s :: state) set)list)). (sl \<noteq> []) \<and>
-                 (sl ! 0, sl ! (length sl - 1)) = (I,s) \<and>
-                 (\<forall> i < (length sl - 1).  \<turnstile> \<N>\<^bsub>(sl ! i,sl ! (i+1) )\<^esub>
-                         )) \<Longrightarrow> \<exists> (A :: ('s :: state) attree).
-                                   \<turnstile> A \<and> attack A = (I,s)"
-  apply (erule disjE)
-  apply (rule_tac x = "([] \<oplus>\<^sub>\<and>\<^bsup>((s,s))\<^esup>)" in exI)  
-   apply simp
-   apply (subst att_and)
-   apply simp
-    apply (erule exE)
-  apply (rule_tac x = 
-"[ \<N>\<^bsub>(sl ! i, sl ! (i + (1::nat)))\<^esub>. i \<leftarrow> [0..<(length sl-(1::nat))]] \<oplus>\<^sub>\<and>\<^bsup>((I,s))\<^esup>" in exI)
-  apply (rule conjI)
-  prefer 2
-   apply simp
-    (*  *) 
-    apply (rule mp)
-    prefer 2
-   apply assumption
-  apply (rule_tac x = I in spec)
-    apply (rule_tac x = s in spec)
-  apply (rule_tac list = sl in list.induct)
+
+(*  lemma finite_set_list:   "finite S \<Longrightarrow>    \<exists>lS::'s list. set lS = S"
+by (rule finite_list)
+  *)
+  
+lemma forall_ex_fun: "finite S \<Longrightarrow> (\<forall> x \<in> S. (\<exists> y. P y x)) \<longrightarrow> (\<exists> f. \<forall> x \<in> S. P (f x) x)"
+  apply (erule finite_induct)
    apply simp
   apply clarify
-  apply simp
-  apply (case_tac "x2 = []")
-   apply simp
-   apply (rule att_and_empty2)
-  apply (drule mp)
+  apply (subgoal_tac "(\<forall>x::'a\<in>F. \<exists>y::'b. P y x)")
+   apply (drule mp)
+    apply assumption
+   apply (erule exE)
+   apply (drule_tac x = x in bspec)
+    apply simp
+    apply (erule exE)
+   apply (rule_tac x = "\<lambda> z. if z = x then y else f z" in exI)
+    apply (rule ballI)
+   apply (erule insertE)
+by simp+
+
+   primrec nodup :: "['a, 'a list] \<Rightarrow> bool"
+  where 
+    nodup_nil: "nodup a [] = True" |
+    nodup_step: "nodup a (x # ls) = (if x = a then (a \<notin> (set ls)) else nodup a ls)"
+
+definition nodup_all:: "'a list \<Rightarrow> bool"
+  where
+    "nodup_all l \<equiv> \<forall> x \<in> set l. nodup x l"
+
+lemma nodup_all_lem[rule_format]: 
+  "nodup_all (x1 # a # l) \<longrightarrow> (insert x1 (insert a (set l)) - {x1}) = insert a (set l)"
+  apply (rule_tac list = l in list.induct)
+by (simp add: nodup_all_def)+
+  
+lemma nodup_all_tl[rule_format]: "nodup_all (x # l) \<longrightarrow> nodup_all l"  
+  apply (rule_tac list = l in list.induct)
+by (simp add: nodup_all_def)+
+
+lemma finite_nodup: "finite I \<Longrightarrow> \<exists> l. set l = I \<and> nodup_all l"  
+  apply (erule finite.induct)
+   apply (rule_tac x = "[]" in exI)
+   apply (simp add: nodup_all_def)
+  apply (erule exE)
+  apply (erule conjE)
+  apply (rule_tac x = "if (a \<in> A) then l else (a # l)" in exI)
+  apply (simp add: nodup_all_def)
+ by blast
+  
+lemma Compl_step3a': "I \<noteq> {} \<Longrightarrow> finite I \<Longrightarrow>
+     ( \<forall> x \<in> I.  x \<in> s \<or> (\<exists> (sl :: ((('s :: state) set)list)). 
+                  (sl \<noteq> []) \<and> (tl sl \<noteq> []) \<and>
+                 (sl ! 0, sl ! (length sl - 1)) = ({x},s) \<and>
+                 (\<forall> i < (length sl - 1).  \<turnstile> \<N>\<^bsub>(sl ! i,sl ! (i+1) )\<^esub>
+                         )) \<Longrightarrow> 
+     (\<exists> lI. set lI = {x :: 's :: state. x \<in> I \<and> x \<notin> s} \<and> (\<exists> Sj :: ((('s :: state) set)list) list. 
+               length Sj = length lI \<and> nodup_all lI \<and>
+            (\<forall> j < length Sj. (((Sj ! j)  \<noteq> []) \<and> (tl (Sj ! j) \<noteq> []) \<and>
+                 ((Sj ! j) ! 0, (Sj ! j) ! (length (Sj ! j) - 1)) = ({lI ! j},s) \<and>
+                 (\<forall> i < (length (Sj ! j) - 1).  \<turnstile> \<N>\<^bsub>((Sj ! j) ! i, (Sj ! j) ! (i+1) )\<^esub>
+                         ))))))"  
+  apply (subgoal_tac "\<exists> lI. set lI = {x::'s \<in> I. x \<notin> s} \<and> nodup_all lI")
+   apply (erule exE)
+   apply (erule conjE)
+   apply (rule_tac x = lI in exI)
    apply (rule conjI)
     apply assumption
-   apply (rule allI)
+    apply (subgoal_tac "\<forall> x \<in> set(lI). (\<exists> sl::'s set list.
+              sl \<noteq> [] \<and>
+              tl sl \<noteq> [] \<and>
+              (sl ! (0::nat), sl ! (length sl - (1::nat))) = ({x}, s) \<and>
+              (\<forall>i<length sl - (1::nat). \<turnstile>\<N>\<^bsub>(sl ! i, sl ! (i + (1::nat)))\<^esub>))")
+    prefer 2
+    apply clarify
+    apply (drule_tac x = x in bspec)
+    apply simp
+    apply (erule disjE)
+     apply simp
+    apply assumption
+    apply (thin_tac " \<forall>x::'s\<in>I.
+          x \<in> s \<or>
+          (\<exists>sl::'s set list.
+              sl \<noteq> [] \<and>
+              tl sl \<noteq> [] \<and>
+              (sl ! (0::nat), sl ! (length sl - (1::nat))) = ({x}, s) \<and>
+              (\<forall>i<length sl - (1::nat). \<turnstile>\<N>\<^bsub>(sl ! i, sl ! (i + (1::nat)))\<^esub>))")
+   apply (subgoal_tac "finite (set lI)")
+    apply (rotate_tac -1)
+   apply (drule forall_ex_fun)
+  apply (drule mp)
+    apply assumption
+apply (thin_tac "\<forall>x::'s\<in>set lI.
+          \<exists>sl::'s set list.
+             sl \<noteq> [] \<and>
+             tl sl \<noteq> [] \<and>
+             (sl ! (0::nat), sl ! (length sl - (1::nat))) = ({x}, s) \<and>
+             (\<forall>i<length sl - (1::nat). \<turnstile>\<N>\<^bsub>(sl ! i, sl ! (i + (1::nat)))\<^esub>)")      
+    apply (erule exE)
+    apply (rule_tac x = "[f (lI ! j). j \<leftarrow> [0..<(length lI)]]" in exI)
+    apply simp
+    apply (rule allI)
+    apply (rule impI)
+    apply (drule_tac x = "lI ! j" in spec)
+    apply (erule mp)
+    apply force
+    thm finite_subset
+     apply (rule_tac A = "set lI" and B = I in finite_subset)
+      apply blast
+      apply assumption
+     apply (subgoal_tac "finite {x::'s \<in> I. x \<notin> s}")
+     apply (rotate_tac -1)
+      apply (erule finite_nodup)
+    apply (rule_tac A = "{x::'s \<in> I. x \<notin> s}" and B = I in  finite_subset)
+     apply blast
+    by assumption
+  
+lemma list_one_tl_empty[rule_format]: "length l = Suc (0 :: nat) \<longrightarrow> tl l = []"
+  apply (rule_tac list = l in list.induct)
+by simp+
+  
+lemma list_two_tl_not_empty[rule_format]: "\<forall> list. length l = Suc (Suc (length list)) \<longrightarrow> tl l \<noteq> []"  
+  apply (rule_tac list = l in list.induct)
+   apply simp+
+by force
+
+lemma or_empty: "\<turnstile> [] \<oplus>\<^sub>\<or>\<^bsup>({}, s)\<^esup>" 
+  by (simp add: att_or)
+    
+(* for any l not valid     
+    lemma or_empty_list: "\<turnstile> l \<oplus>\<^sub>\<or>\<^bsup>({}, s)\<^esup>" 
+*)
+      
+lemma list_or_upt[rule_format]: 
+ "\<forall> l . lI \<noteq> [] \<longrightarrow> length l = length lI \<longrightarrow> nodup_all lI \<longrightarrow>
+  (\<forall> i < length lI. (\<turnstile> (l ! i)) \<and> (attack (l ! i) = ({lI ! i}, s))) 
+                \<longrightarrow> ( \<turnstile> (l \<oplus>\<^sub>\<or>\<^bsup>(set lI, s)\<^esup>))"     
+  apply (rule_tac list = lI in list.induct)
+   apply simp
+  apply clarify
+  apply (case_tac x2)
+    apply simp
+   apply (subst att_or)
+    apply simp
+  apply clarify
+  apply (rule conjI)
+    apply clarify
+    apply (rule conjI)
+     apply force
+    apply (rule impI)
+   apply (subst hd_conv_nth, assumption)+
+    apply simp
+   apply clarify
+   apply (rule conjI)
+    apply force
+    apply (rule impI)
+    apply (subst hd_conv_nth, assumption)
+   apply (rule conjI)
+    apply assumption
+    apply (subst hd_conv_nth, assumption)
+    apply simp
+    apply (rule conjI)
+   apply (drule list_one_tl_empty)
+   apply (erule notE, assumption)
+    (* x2 \<noteq> [] *)
+    apply (drule list_one_tl_empty)
+   apply (erule notE, assumption)
+      apply (subst att_or)
+  apply simp
+  apply clarify
+    apply (rule conjI)
    apply (rule impI)
+    apply (rule conjI)
+    apply force
+   apply (rule impI)
+   apply (drule list_two_tl_not_empty)
+   apply (erule notE, assumption)
+  apply (rule impI)
+  apply (rule conjI)
+   apply force
+  apply (rule impI)
+    apply (rule conjI)
+    apply (rotate_tac -3)
+    apply (drule_tac x = 0 in spec)
+    apply (drule mp)
+     apply simp
+    apply (erule conjE)+
+    apply (subst hd_conv_nth, assumption)
+     apply simp
+  apply (rule conjI)
+     apply (subst hd_conv_nth, assumption)
    apply (rotate_tac -3)
-   apply (drule_tac x = "i + 1" in spec)
+   apply (drule_tac x = 0 in spec)
+   apply (drule mp)
+    apply simp
+   apply (erule conjE)
+    apply (rotate_tac -1)
+    apply (erule ssubst)
+   apply simp
+  apply (rule conjI)
+    apply (subst hd_conv_nth, assumption)
+     apply (rotate_tac -3)
+   apply (drule_tac x = 0 in spec)
+   apply (drule mp)
+    apply simp
+   apply (erule conjE)
+   apply (rotate_tac -1)
+    apply (erule ssubst)
+   apply simp
+    (* tl instance !*)
+  apply (drule_tac x  = "tl l" in spec)
+  apply (drule mp)
+    apply simp
+  apply (drule mp)
+   apply (erule nodup_all_tl)
+    apply (drule mp)
+   apply (rule allI)
+  apply (rule impI)
+   apply (drule_tac x = "Suc i" in spec)
    apply (drule mp)
     apply arith
+   apply (rule conjI)
+    apply (erule conjE)
+    apply (subgoal_tac "l ! Suc i = tl l ! i")
+     apply (erule subst, assumption)
+    apply (case_tac l)
+     apply (erule notE, assumption)
+    apply simp+
+    apply (erule conjE)
+    apply (subgoal_tac "l ! Suc i = tl l ! i")
+     apply (erule subst, assumption)
+    apply (case_tac l)
+    apply (erule notE, assumption)
+   apply simp
+  apply (subst hd_conv_nth, assumption)
+    apply (frule_tac x = 0 in spec)
+   apply (drule mp)
+   apply simp
+    (* additional assumption nodup (x1 # a # list) to show that
+       (insert x1 (insert a (set list)) - fst (attack (l ! (0::nat))) = insert a (set list)
+        given that fst(attack (l ! 0)) = {x1} *)
+  apply (subgoal_tac "fst (attack (l ! (0::nat))) = {x1}")
+   apply (rotate_tac -1)
+    apply (erule ssubst)
+  apply (subst nodup_all_lem,assumption,assumption)
+by simp
+        
+lemma app_tl_empty_hd[rule_format]: "tl (l @ [a]) = [] \<longrightarrow> hd (l @ [a]) = a"
+  apply (rule_tac list = l in list.induct)
+by simp+
+       
+lemma tl_hd_empty[rule_format]: "tl (l @ [a]) = [] \<longrightarrow> l = []"
+    apply (rule_tac list = l in list.induct)
+by simp+
+
+lemma tl_hd_not_empty[rule_format]: "tl (l @ [a]) \<noteq> [] \<longrightarrow> l \<noteq> []"
+    apply (rule_tac list = l in list.induct)
+by simp+
+  
+lemma app_tl_empty_length[rule_format]: "tl (map f [0::nat..<length l] @ [a]) = []  
+                                        \<Longrightarrow> l = []"
+  apply (drule tl_hd_empty)
+by simp
+  
+lemma not_empty_hd_fst[rule_format]: "l \<noteq> [] \<longrightarrow> hd(l @ [a]) = l ! 0"
+  apply (rule_tac list = l in list.induct)
+by simp+
+  
+lemma app_tl_hd_list[rule_format]: "tl (map f [0::nat..<length l] @ [a]) \<noteq> []  
+                             \<Longrightarrow> hd(map f [0::nat..<length l] @ [a]) = (map f [0::nat..<length l]) ! 0"
+  apply (drule tl_hd_not_empty)
+by (erule not_empty_hd_fst)
+  
+lemma tl_app_in[rule_format]: "l \<noteq> [] \<longrightarrow>
+   map f [0::nat..<(length l - (Suc 0:: nat))] @ [f(length l - (Suc 0 :: nat))] = map f [0::nat..<length l]"    
+  apply (rule_tac list = l in list.induct)
+  by simp+
+    
+lemma map_fst[rule_format]: "n > 0 \<longrightarrow> map f [0::nat..<n] = f 0 # (map f [1..<n])"
+  apply (induct_tac n)
+   apply simp
+    apply (case_tac n)
+by simp+
+    
+lemma step_lem[rule_format]:  "l \<noteq> [] \<Longrightarrow>
+       tl (map (\<lambda> i. f((x1 # a # l) ! i)((a # l) ! i)) [0::nat..<length l]) =
+       map (\<lambda>i::nat. f((a # l) ! i)(l ! i)) [0::nat..<length l - (1::nat)]"
+  apply simp
+  apply (subgoal_tac "map (\<lambda>i::nat. f ((x1 # a # l) ! i) ((a # l) ! i)) [0::nat..<length l] =
+                 (f(x1)(a) # (map (\<lambda>i::nat. f ((a # l) ! i) (l ! i)) [0::nat..<(length l - 1)]))")
+   apply (erule ssubst)
+   apply simp
+  apply (subgoal_tac "map (\<lambda>i::nat. f ((x1 # a # l) ! i) ((a # l) ! i)) [0::nat..<length l] =
+                     f ((x1 # a # l) ! 0) ((a # l) ! 0) # 
+                     (map (\<lambda>i::nat. f ((x1 # a # l) ! i) ((a # l) ! i)) [1::nat..<length l])")
+   apply (erule ssubst)
+    apply simp
+  apply (subgoal_tac "map (\<lambda>i::nat. f ((x1 # a # l) ! i) ((a # l) ! i)) [Suc (0::nat)..<length l] =
+             map (\<lambda>i::nat. f ((x1 # a # l) ! Suc i) ((a # l) ! Suc i)) [(0::nat)..<(length l - 1)]")
+    apply simp
+    apply (subgoal_tac "[Suc (0::nat)..<length l] = map Suc [0..<(length l - 1)]")
+    apply (erule ssubst)
+    apply simp
+   apply (simp add: map_Suc_upt)
+  apply (rule map_fst)
+by simp
+  
+lemma base_list_and[rule_format]: "Sji \<noteq> [] \<longrightarrow> tl Sji \<noteq> [] \<longrightarrow>
+         (\<forall> li.  Sji ! (0::nat) = li \<longrightarrow>
+        Sji! (length (Sji) - 1) = s \<longrightarrow>
+       (\<forall>i<length (Sji) - 1. \<turnstile>\<N>\<^bsub>(Sji ! i, Sji ! Suc i)\<^esub>) \<longrightarrow>
+       \<turnstile>map (\<lambda>i::nat. \<N>\<^bsub>(Sji ! i, Sji ! Suc i)\<^esub>)
+          [0::nat..<length (Sji) - Suc (0::nat)] \<oplus>\<^sub>\<and>\<^bsup>(li, s)\<^esup>)"
+
+  apply (rule_tac list = Sji in list.induct)
+    apply simp
+  apply (subst att_and)
+  apply (case_tac x2)
    apply simp
   apply simp
-  apply (subgoal_tac "(map (\<lambda>i::nat. \<N>\<^bsub>((x1 # x2) ! i, x2 ! i)\<^esub>) [0::nat..<length x2]) = 
-                      \<N>\<^bsub>(x1, x2 ! 0)\<^esub> # (map (\<lambda>i::nat. \<N>\<^bsub>(x2 ! i, x2 ! Suc i)\<^esub>)[0::nat..<length x2 - Suc (0::nat)])")
-  apply (rotate_tac -1)
-   apply (erule ssubst)
-   apply (rule att_comp_and_cons)
-     apply (rotate_tac -3)
-     apply (drule_tac x = 0 in spec)
-     apply simp
+ (*   apply (rule allI) *)
+  apply (rule conjI)
+   apply (rule impI)+
+    apply (rule conjI)
+    apply (drule_tac x = "length list" in spec)
+    apply (subst app_tl_empty_hd,assumption)
     apply simp
-   apply assumption
-  apply (subgoal_tac " map (\<lambda>i::nat. \<N>\<^bsub>((x1 # x2) ! i, x2 ! i)\<^esub>) [0::nat..<length x2] =
-                       \<N>\<^bsub>(x1, x2 ! (0::nat))\<^esub> #
-                        map (\<lambda>i::nat. \<N>\<^bsub>((x1 # x2) ! Suc i, x2 ! Suc i)\<^esub>) [0::nat..<length x2 - 1]")
+   apply (subgoal_tac "length list = 0")
+    apply simp
+   apply (drule app_tl_empty_length)
    apply simp
-  apply (subgoal_tac "map (\<lambda>i::nat. \<N>\<^bsub>((x1 # x2) ! Suc i, x2 ! Suc i)\<^esub>) [0::nat..<length x2 - (1::nat)]
-                   = map (\<lambda>i::nat. \<N>\<^bsub>((x1 # x2) ! i, x2 ! i)\<^esub>) [1::nat..<length x2]")
-   apply (rotate_tac -1)
-   apply (erule ssubst)
-   apply (subgoal_tac "x1 = (x1 # x2) ! 0")
+(* *)
+  apply clarify
+  apply (rule conjI)
+   apply (subst app_tl_hd_list, assumption)
+   apply simp
+   apply (subst nth_map)
+    apply force
+   apply (drule_tac x = 0 in spec)
+   apply (subgoal_tac "[0::nat..<length list] ! (0::nat) = 0")
+    apply simp
+   apply (drule tl_hd_not_empty)
+   apply (subgoal_tac "0 < length list")
+    apply simp+
+(* *)
+  apply (rule conjI)
+    apply (subst app_tl_hd_list)
+    apply simp
+   apply (subst nth_map)
+    apply force
+    apply simp
+   apply (subgoal_tac "[0::nat..<length list] ! (0::nat) = 0")
+    apply simp
+     apply (drule tl_hd_not_empty)
+   apply (subgoal_tac "0 < length list")
+    apply simp
+    apply simp
+    (* *)
+  apply (drule mp)
+   apply (drule tl_hd_not_empty)
+   apply simp
+  apply (subst not_empty_hd_fst)
+   apply (erule tl_hd_not_empty)
+  apply (drule mp)
+   defer
+apply (subgoal_tac "map (\<lambda>i::nat. \<N>\<^bsub>((a # list) ! i, list ! i)\<^esub>)
+          [0::nat..<length list] = tl (map (\<lambda>i::nat. \<N>\<^bsub>((x1 # a # list) ! i, (a # list) ! i)\<^esub>) [0::nat..<length list] @
+             [\<N>\<^bsub>((x1 # a # list) ! length list,
+                  (a # list) !
+                  length
+                   list)\<^esub>])")
     apply (rotate_tac -1)
-    apply (rule_tac P = "(\<lambda> y. map (\<lambda>i::nat. \<N>\<^bsub>((x1 # x2) ! i, x2 ! i)\<^esub>) [0::nat..<length x2] =
-       \<N>\<^bsub>(y, x2 ! (0::nat))\<^esub> # map (\<lambda>i::nat. \<N>\<^bsub>((x1 # x2) ! i, x2 ! i)\<^esub>) [1::nat..<length x2])" 
-      in ssubst)
-     apply assumption
-    apply (rule sym)
-    apply (rule map_hd_lem)
+    apply (erule subst)
+    apply (subgoal_tac "snd (attack
+                              (map (\<lambda>i::nat. \<N>\<^bsub>((x1 # a # list) ! i, (a # list) ! i)\<^esub>)
+                                [0::nat..<length list] !
+                               (0::nat))) = a")
+  apply (rotate_tac -1)
+     apply (erule ssubst)
+     apply (subgoal_tac "(a # list) ! length list = list ! (length list - Suc (0::nat))")
+      apply (rotate_tac -1)
+      apply (erule ssubst)
+      apply assumption
+     apply (subgoal_tac "list \<noteq> []")
+      apply simp
+     apply (frule tl_hd_not_empty)
+     apply simp
+    apply (subgoal_tac "list \<noteq> []")
+     apply simp
+    apply (frule tl_hd_not_empty)
+    apply simp
+    apply (subgoal_tac "list \<noteq> []")
+    apply simp
+  apply (subgoal_tac "tl (map (\<lambda>i::nat. \<N>\<^bsub>((x1 # a # list) ! i, (a # list) ! i)\<^esub>) [0::nat..<length list])
+                     =  (map (\<lambda>i::nat. \<N>\<^bsub>((a # list) ! i, (list) ! i)\<^esub>) [0::nat..<(length list - 1)])")
+     apply simp
+     apply (rule sym)
+     apply (erule tl_app_in)
+    apply (erule step_lem)
+(* bla *)
+   apply force
+by force    
+    
+ lemma Compl_step3b: "I \<noteq> {} \<Longrightarrow> finite I \<Longrightarrow> \<not> I \<subseteq> s \<Longrightarrow>
+(\<exists> lI. set lI = {x. x \<in> I \<and> x \<notin> s} \<and> (\<exists> Sj :: ((('s :: state) set)list) list. 
+               length Sj = length lI \<and> nodup_all lI \<and>
+            (\<forall> j < length Sj. (((Sj ! j)  \<noteq> []) \<and> (tl (Sj ! j) \<noteq> []) \<and>
+                 ((Sj ! j) ! 0, (Sj ! j) ! (length (Sj ! j) - 1)) = ({lI ! j},s) \<and>
+                 (\<forall> i < (length (Sj ! j) - 1).  \<turnstile> \<N>\<^bsub>((Sj ! j) ! i, (Sj ! j) ! (i+1) )\<^esub>
+                         )))))
+ \<Longrightarrow>  \<exists> (A :: ('s :: state) attree).  \<turnstile> A \<and> attack A = (I,s)"
+   apply (erule exE)
+   apply (erule conjE)
+   apply (erule exE)
+   apply (erule conjE)
+     apply (rule_tac x = 
+ "[([] \<oplus>\<^sub>\<or>\<^bsup>({x. x \<in> I \<and> x \<in> s}, s)\<^esup>),
+    ([[ \<N>\<^bsub>((Sj ! j) ! i, (Sj ! j) ! (i + (1::nat)))\<^esub>. 
+      i \<leftarrow> [0..<(length (Sj ! j)-(1::nat))]] \<oplus>\<^sub>\<and>\<^bsup>(({lI ! j},s))\<^esup>. j \<leftarrow> [0..<(length Sj)]]
+     \<oplus>\<^sub>\<or>\<^bsup>({x. x \<in> I \<and> x \<notin> s},s)\<^esup>)] \<oplus>\<^sub>\<or>\<^bsup>(I, s)\<^esup>" in exI)
+   apply (rule conjI)
+   prefer 2
+    apply simp
+   apply (subst att_or)
+   apply simp
+   apply (rule conjI)
+       apply (subst att_or)
+    apply simp
+   apply (rule subsetI)
+    apply (drule CollectD)
+     apply (erule conjE, assumption)
+   apply (rule conjI)
+    apply (rule subsetI)
+    apply (drule CollectD)
+    apply (erule conjE, assumption)
+   apply (subgoal_tac "I - {x::'s \<in> I. x \<in> s} = {x::'s \<in> I. x \<notin> s}")
+   apply (rotate_tac -1)
+     apply (erule ssubst)
+   apply (subst att_or)
+    apply simp
+   prefer 2
+    apply blast
+   apply (rule subst, assumption)
+     (* induction over list lI *)
+   apply (rule_tac lI = lI in list_or_upt)
+     (* fst (attack (l ! (0::nat))) *)
+    apply (subgoal_tac "set lI \<noteq> {}")
+     apply force
+    apply (erule ssubst)
+    apply (subgoal_tac "\<exists> x. x \<in> I \<and> x \<notin> s")
+     apply (erule exE)
+     apply blast
+    apply blast
+     apply simp
+     apply (erule conjE, assumption)
+   apply (rule conjI)
+   prefer 2
     apply simp
    apply simp
-  apply (rule sym)
-  apply (rule map_Suc_lem)
-    by simp
-
-theorem Completeness: "I \<noteq> {} \<Longrightarrow> Kripke {s :: ('s :: state). \<exists> i \<in> I. (i \<rightarrow>\<^sub>i* s)} (I :: ('s :: state)set)  \<turnstile> EF s 
+     apply (erule conjE)
+   apply (drule_tac x = i in spec)
+   apply (drule mp, assumption)
+   apply (rule base_list_and)
+     apply (erule conjE)+
+       apply assumption
+     apply (erule conjE)+
+       apply assumption
+     apply (erule conjE)+
+       apply assumption
+     apply (erule conjE)+
+    apply simp
+   apply (erule conjE)+
+     apply (drule spec, erule mp)
+     by simp
+       
+theorem Completeness: "I \<noteq> {} \<Longrightarrow> finite I \<Longrightarrow> 
+Kripke {s :: ('s :: state). \<exists> i \<in> I. (i \<rightarrow>\<^sub>i* s)} (I :: ('s :: state)set)  \<turnstile> EF s 
 \<Longrightarrow> \<exists> (A :: ('s :: state) attree).
                                    \<turnstile> A \<and> attack A = (I,s)"
-  apply (rule Compl_step3)
-  apply (erule Compl_step2)
+  apply (case_tac "I \<subseteq> s")
+   apply (rule_tac x = "((([] :: ((('s :: state) attree) list)) \<oplus>\<^sub>\<and>\<^bsup>(I,s)\<^esup>))" in exI)
+   apply (subst att_and)
+   apply simp
+  apply (rule Compl_step3b)
+    apply assumption+
+  apply (rule Compl_step3a')
+    apply assumption+
+  apply (rule Compl_step2)
   by (erule Compl_step1)
     
 end
